$\int f'(g(x)) * g'(x) dx = f(g(x))$

# Integral Substitution 
$\int f(x)dx = \int f(g(t)) * g'(t) dt\ |\ t = g^{-1}(x)$ 

## Trigonometric Functions
**Mivel** $\cos^2(\alpha) = \frac{1}{1+\tan^2(\alpha)}$
- $\sin(x) = \frac{2*\tan\left( \frac{x}{2} \right)}{1+\tan^2\left( \frac{x}{2} \right)} = \frac{2t}{1+t^2}$ 
- $\cos(x) = \frac{1-\tan^2\left( \frac{x}{2} \right)}{1+\tan^2\left( \frac{x}{2} \right)} = \frac{1-t^2}{1+t^2}$ 
*ahol*:
- $t = \tan\left( \frac{x}{2} \right)$ (néha $t=\tan(x)$ is megjelenhet tetszés szerint)
*ekkor* persze:
- $g(t) = 2 \arctan(t) = x$  
- $dx = \frac{2}{1+t^2}$

# Partial Integration 
$(f*g)' = f'*g + f*g' \implies \int (f*g)' =\int f'*g + \int f*g' \implies \int f*g' = f*g - \int f'*g$

# Solving Integrals using Equations