# Trigonometric formulas
- $\sin(-x) = -\sin(x)$
- $\cos(-x) = \cos(x)$
# Addiciós tételek

$\sin(\alpha \pm \beta) = \sin \alpha * \cos\beta \pm \cos \alpha*\sin \beta$
$\cos(\alpha\pm \beta) = \cos \alpha*\cos \beta \mp \sin \alpha*\sin \beta$

## Felhasználás:
### $\sin * \cos$ 
- $\sin(\alpha+ \beta) =\sin \alpha *\cos \beta + \cos \alpha *\sin \beta$ 
- $\sin(\alpha - \beta) = \sin \alpha * \cos \beta - \cos \alpha * \sin \beta$
- $\implies (I.- II.)$
- $2*\sin \beta*\cos \alpha =\sin(\alpha + \beta) - \sin(\alpha - \beta)$
## $\cos * \cos$
- $\cos(\alpha + \beta) = \cos \alpha*\cos \beta - \sin \alpha * \sin \beta$
- $\cos(\alpha - \beta) = \cos \alpha * \cos \beta + \sin \alpha * \sin \beta$
- $\implies (I. + II.)$
- $2*\cos \alpha * \cos \beta = \cos (\alpha + \beta) + \cos(\alpha-\beta)$
## $\sin * \sin$
- $\cos(\alpha + \beta) = \cos \alpha*\cos \beta - \sin \alpha * \sin \beta$
- $\cos(\alpha - \beta) = \cos \alpha * \cos \beta + \sin \alpha * \sin \beta$
- $\implies (I. - II.)$
- $-2*\sin \alpha * \sin \beta = \cos (\alpha + \beta) - \cos(\alpha-\beta)$